% \documentclass[tikz,convert={outfile=\jobname.svg}]{standalone}
\documentclass[crop,equation,convert={outext=,command=\unexpanded{pdf2svg \infile\space ./LatexPics/LatexPic-\%d.svg all}},multi=alone]{standalone}
% \documentclass{article}
\usepackage{amsmath}
\input{tikzMacros.tex}
\usetikzlibrary{arrows.meta}
\tikzset{
    side by side/.style 2 args={
    line width=2pt,
    #1,
    postaction={
        clip,postaction={draw,#2, line width=6pt}
        }
    }
}
\tikzstyle{treeNode}[black]=[draw=#1,fill=#1!20, circle, inner sep = 5pt]
\tikzstyle{treeNodeLabeled}[black]=[draw=#1, circle, inner sep = 1pt]
\tikzstyle{treeNodeMarked}[red]=[draw=#1,fill=#1!20, circle, inner sep = 5pt]%, edge=treeEdgeMarked]
\tikzstyle{treeNodeInner}=[inner sep = 0pt, circle, fill]
% \tikzstyle{treeNodeRoot}=[draw, inner sep = 3pt]
\tikzstyle{treeNodeRoot}=[inner sep = 2pt, circle, fill]
\tikzstyle{treeEdgeMarked}=[red, very thick]
\tikzstyle{treeEdgeDouble}=[side by side={red!50}{blue!50}]

% \usepackage[margins=0]{geometry}
\usepackage{ytableau}
\usepackage{forest}

\begin{document}
\color{black}

\forestset{
  default preamble={
      for tree={l = 0cm, s sep = 0.5cm,calign=fixed edge angles}
    }
}
\Large
% \boldmath
\begin{alone}
  \begin{forest}
    [, treeNodeRoot
        [, treeNode]
        [, treeNodeInner
            [, treeNodeInner
                [, treeNode]
                [, treeNode]
            ]
            [, treeNodeInner
                [, treeNode]
                [, treeNode]
            ]
        ]
    ]
  \end{forest}
\end{alone}
\begin{alone}
  \begin{forest}
    [, treeNodeRoot
        [, treeNodeMarked]
        [, treeNodeInner
            [, treeNodeInner
                [, treeNode]
                [, treeNodeMarked]
            ]
            [, treeNodeInner
                [, treeNodeMarked]
                [, treeNode]
            ]
        ]
    ]
  \end{forest}
\end{alone}
\begin{alone}
  \begin{forest}
    [, treeNodeRoot
    [, treeNodeMarked, edge=treeEdgeMarked]
    [, treeNodeInner, edge=treeEdgeMarked
    [, treeNodeInner, edge=treeEdgeMarked
    [, treeNode]
    [, treeNodeMarked, edge=treeEdgeMarked]
    ]
    [, treeNodeInner, edge=treeEdgeMarked
    [, treeNodeMarked, edge=treeEdgeMarked]
    [, treeNode]
    ]
    ]
    ]
  \end{forest}
\end{alone}
\begin{alone}
  \begin{forest}
    [, treeNodeRoot
    [, treeNodeMarked, edge=treeEdgeMarked]
    [, treeNodeInner, edge=treeEdgeMarked
    [, treeNodeInner, edge=treeEdgeMarked
    [, treeNodeMarked, edge=treeEdgeMarked]
    ]
    [, treeNodeInner, edge=treeEdgeMarked
    [, treeNodeMarked, edge=treeEdgeMarked]
    ]
    ]
    ]
  \end{forest}
\end{alone}
\begin{alone}
  \begin{forest}
    [, treeNodeRoot
        [, treeNode]
        [, treeNodeInner
            [, treeNode]
            [, treeNode]
        ]
    ]
  \end{forest}
\end{alone}
\begin{alone}
  $\mathrm{ex}\left(\FlagGraph[very thick,darkorange]{2}{1--2};\raisebox{-2pt}{\FlagGraph[very thick,darkgreen]{3}{1--2,2--3,1--3}}\right)\coloneqq \max_\mathcal{G} \left\lbrace \phi\left(\FlagGraph[very thick,darkorange,scale=1]{2}{1--2}\right) : \phi\left(\raisebox{-2pt}{\FlagGraph[very thick,darkgreen]{3}{1--2,2--3,1--3}}\right) = 0\right\rbrace.$
\end{alone}
\begin{alone}
  $\mathrm{ex}\left(\FlagGraph[very thick,darkorange]{2}{1--2};\raisebox{-2pt}{\FlagGraph[very thick,darkgreen]{3}{1--2,2--3,1--3}}\right) \geq \frac{1}{2},$
\end{alone}
\begin{alone}
  $\phi\left(\FlagGraph{2}{1--2}\right)  \phi\left(\raisebox{-2pt}{\FlagGraph{3}{1--2,2--3,1--3}}\right) = \phi\left(\raisebox{-0pt}{\FlagGraph{5}{1--2,3--4,4--5,3--5}}\right).$
\end{alone}
\begin{alone}
  $\FlagGraph{2}{1--2}\cdot\FlagGraph{3}{1--2,2--3,1--3}=  \FlagGraph{5}{1--2,3--4,4--5,3--5},$
\end{alone}
\begin{alone}
  $\FlagGraphNumb{3}{1--2,2--3,1--3}{2} \cdot \FlagGraphNumb{3}{1--2,1--3}{1} = \FlagGraphNumb{5}{1--2,1--3,2--3,1--4,1--5}{2}$
\end{alone}
\begin{alone}
  $\left(1 \varnothing - 2\FlagGraphNumb{2}{1--2}{1}\right)^2 = \varnothing -4\FlagGraphNumb{2}{1--2}{1}+4\FlagGraphNumb{3}{1--2,1--3}{1}\geq 0.$
\end{alone}
\begin{alone}
  $\left\llbracket \left(1 \varnothing - 2\FlagGraphNumb{2}{1--2}{1}\right)^2 \right\rrbracket = \varnothing - 4\FlagGraph{2}{1--2} + 4\FlagGraph{3}{1--2,1--3}\geq 0.$
\end{alone}
\begin{alone}
  $\frac{1}{2} - \FlagGraph{2}{1--2} =  \left\llbracket \frac{1}{2} \left(1 \varnothing - 2\FlagGraphNumb{2}{1--2}{1}\right)^2 \right\rrbracket\\
    + \left\llbracket \left(\FlagGraphNumb{2}{1--2}{2} - \FlagGraphNumb{3}{1--2,2--3}{3} - \FlagGraphNumb{3}{1--2, 1--3}{3} + \FlagGraphNumb{3}{1--2,1--3,2--3}{3}\right)^2 \right\rrbracket\\
    -\FlagGraph{3}{1--2,1--3,2--3} \geq 0.$
\end{alone}
\begin{alone}
  $\llbracket f^2 \rrbracket = \langle cc^\top, \llbracket{\color{darkorange}\mathcal{F}}{\color{darkorange}\mathcal{F}}^\top\rrbracket\rangle$
\end{alone}
\begin{alone}
  $\langle M, \llbracket{\color{darkorange}\mathcal{F}}{\color{darkorange}\mathcal{F}}^\top\rrbracket\rangle$
\end{alone}
\begin{alone}
  $H - \FlagGraph{2}{1--2}^{|E(H)|} \geq 0.$
\end{alone}
\begin{alone}
  $\nabla_{\color{orange}v} f(x) = \lim_{{\color{red}h}\to 0}\frac{f(x+{\color{red}h}{\color{orange}v})-f(x)}{{\color{red}h}}$
\end{alone}
\begin{alone}
  $\partial_{\color{orange}v} H :=\lim_{{\color{red}i}\to\infty}\frac{(H \text{ density in
    }(G_{\color{red}i}-{\color{orange}v})) - (H \text{ density in }G_{\color{red}i})}{{\color{red}i}^{-1}}$
\end{alone}
\begin{alone}
  $\substack{\partial_1 \FlagGraph{2}{1--2} \enspace = \enspace 2\FlagGraph{2}{1--2} - 2\FlagGraphNumb{2}{1--2}{1}\\\vspace{1cm}\\ \partial_1 \FlagGraph{3}{1--2,1--3} \enspace = \enspace 3\FlagGraph{3}{1--2,1--3} - 2\FlagGraphLabelThree{1--2,1--3}{0}{1}{0} - \FlagGraphLabelThree{1--2,1--3}{1}{0}{0}}$
\end{alone}
\begin{alone}
  $\partial_{\color{orange}e} H :=\lim_{{\color{red}i}\to\infty}\frac{(H \text{ density in
  }(G_{\color{red}i}-{\color{orange}e})) - (H \text{ density in }G_{\color{red}i})}{{\color{red}i}^{-2}}$
\end{alone}
\begin{alone}
  $\substack{\partial_e \FlagGraph{2}{1--2} \enspace=\enspace - 2\FlagGraphNumb{2}{1--2}{2} \\\vspace{0.5cm}\\
  \partial_e \FlagGraph{3}{1--2,1--3} \enspace=\enspace - 2\FlagGraphLabelThree{1--2,1--3}{2}{1}{0} - 2\FlagGraphLabelThree{1--2,1--3}{1}{2}{0} 
  \\\vspace{0.5cm}\\\partial_e \FlagGraph{3}{1--2,1--3,2--3} \enspace=\enspace - 6 \FlagGraphLabelThree{1--2,1--3,2--3}{1}{2}{0}}$
\end{alone}
\begin{alone}
$\left\llbracket\FlagGraphLabelTwo{1--2}{1}{3}\partial_{\text{swap}}(P_3-e^3)\right\rrbracket = \FlagGraph{6}{1--2,2--3,4--5,5--6} + \FlagGraph{6}{1--2,2--3,3--4,5--6}-2\FlagGraph{5}{1--2,2--3,2--5,4--5}\geq 0$

% \bigg\llbracket \FlagGraphLabelTwo{1--2}{1}{3}\bigg(2\FlagGraphLabelFive{1--2, 3--4,4--5}{4}{3}{2}{0}{0}+2\FlagGraphLabelFive{1--2, 3--4,4--5}{4}{3}{1}{0}{0}+2\FlagGraphLabelFive{1--2, 3--4,4--5}{2}{1}{3}{0}{0}+2\FlagGraphLabelFive{1--2, 3--4,4--5}{2}{1}{4}{0}{0}+2\FlagGraphLabelSix{1--2,3--4,5--6}{4}{3}{1}{0}{0}{2}+2\FlagGraphLabelSix{1--2,3--4,5--6}{2}{1}{3}{4}{4}{4}\\\qquad
% -2\FlagGraphLabelFour{1--2,2--3,3--4}{1}{2}{0}{0}-2\FlagGraphLabelFour{1--2,2--3,3--4}{2}{1}{0}{0}-2\FlagGraphLabelFour{1--2,2--3,3--4}{3}{4}{0}{0}-2\FlagGraphLabelFour{1--2,2--3,3--4}{4}{3}{0}{0}-2\FlagGraphLabelFour{1--2,2--3,3--4}{0}{1}{2}{0}-2\FlagGraphLabelFour{1--2,2--3,3--4}{0}{3}{4}{0}\bigg)\bigg\rrbracket$
\end{alone}
\begin{alone}
  But $\FlagGraph{5}{1--2,2--3,2--5,4--5} - \FlagGraph{6}{1--2,2--3,4--5,5--6} = \text{SOS}\geq 0$ and $\FlagGraph{5}{1--2,2--3,2--5,4--5} - \FlagGraph{6}{1--2,2--3,3--4,5--6}= \text{SOS}\geq 0$.
\end{alone}
\begin{alone}
  Thus $\FlagGraph{5}{1--2,2--3,2--5,4--5} = \FlagGraph{6}{1--2,2--3,4--5,5--6} = \FlagGraph{6}{1--2,2--3,3--4,5--6}$.
\end{alone}
\begin{alone}
  This proves $\FlagGraph{6}{1--2,2--3,3--4,5--6} = \FlagGraph{6}{1--2,2--3,4--5,5--6} \geq \FlagGraph{8}{1--2,3--4,5--6,7--8}$.
\end{alone}


\end{document}